Saved predicates using sigT

theories/hoInterps_experiments.v
@@ -1,6 +1,11 @@
 From iris.proofmode Require Import tactics.
 From iris.base_logic Require Import lib.saved_prop.
-From D Require iris_prelude saved_interp_n.
+From D Require Import prelude iris_prelude saved_interp_n.
+
+Unset Program Cases.
+(* Repeat temporarily-disabled Iris notations. *)
+Notation "{ x  &  P }" := (sigTOF (λ x, P%OF)) : oFunctor_scope.
+Notation "{ x : A &  P }" := (@sigTOF A%type (λ x, P%OF)) : oFunctor_scope.
 
 Module try1.
 Section saved_pred3_use.
@@ -29,14 +34,18 @@ Section saved_pred3_use.
 End saved_pred3_use.
 End try1.
 
-Notation savedPred3G Σ A B C := (savedAnythingG Σ (A -d> B -d> C -d> ▶ ∙)).
-Notation savedPred3Σ A B C := (savedAnythingΣ (A -d> B -d> C -d> ▶ ∙)).
-
 Module try2.
 
+Definition vec n vl := fin n → vl.
+
+(* To prove saved_pred3_own_contractive, below, we need to hide n under ▶. *)
+Definition nFun vl : oFunctor := { n & vec n vl -d> (var → vl) -d> vl -d> ∙ }.
+Definition mFun vl : oFunctor := ▶ nFun vl.
+Notation savedPred3G Σ vl := (savedAnythingG Σ (mFun vl)).
+Notation savedPred3Σ vl := (savedAnythingΣ (mFun vl)).
+
 Section saved_pred3.
-  Definition vec n vl := fin n → vl.
-  Context {vl : Type}.
+  Context `{!savedPred3G Σ vl}.
 
   (* vector operations, on a functional representation of vectors. *)
   Definition vcons {n} (v : vl) (args: vec n vl) : fin (S n) → vl :=
@@ -51,8 +60,6 @@ Section saved_pred3.
   Definition vtail {n} (args: vec (S n) vl) : fin n → vl :=
     λ i, args (Fin.FS i).
 
-  Context `{!savedPred3G Σ (var → vl) vl (list vl)}.
-
   Notation envD Σ := ((var → vl) -d> vl -d> iProp Σ).
   Notation hoEnvND n Σ := (vec n vl -d> envD Σ).
   (* Manipulate *)
@@ -66,23 +73,78 @@ Section saved_pred3.
 
   Definition hoEnvD Σ := { n : nat & hoEnvND n Σ }.
 
-  Context `{!savedPred3G Σ A B C}.
+  (* Make hoEnvD a Cofe. *)
+  Definition hoEnvDC Σ : ofeT := sigTC (λ n, hoEnvND n Σ).
+  Global Instance: Cofe (hoEnvDC Σ) := _.
+
   Implicit Types (Φ : hoEnvD Σ).
 
-  (* Argh. hoEnvD isn't a functor. *)
-  (* Definition saved_pred3_own (γ : gname) Φ :=
-    saved_anything_own
-      (F := A -d> B -d> C -d> ▶ ∙) γ (λ a b c, Next (Φ a b c)). *)
-(*
+  Definition packedFun := nFun vl (iProp Σ) uPred_cofe.
+  Definition pack : hoEnvD Σ → laterO packedFun :=
+    λ '(existT n Φ), Next (existT n (λ args ρ v, Φ args ρ v)).
+
+  Definition packedFun_arity : packedFun → nat := projT1.
+  Definition unpack : ∀ (Φ : packedFun), hoEnvND (packedFun_arity Φ) Σ := projT2.
+
+  Definition saved_pred3_own (γ : gname) (Φ : hoEnvD Σ) : iProp Σ :=
+    saved_anything_own (F := mFun vl) γ (pack Φ).
+
   Instance saved_pred3_own_contractive γ : Contractive (saved_pred3_own γ).
-  Proof. rewrite /saved_pred3_own /saved_anything_own. solve_contractive_ho. Qed.
+  Proof. rewrite /saved_pred3_own => n [ix x] [iy y] /= Heq. f_equiv. done. Qed.
+
+  Import uPred EqNotations.
+  Instance: NonExpansive (projT1 : packedFun → nat). solve_proper. Qed.
 
   Lemma saved_pred3_alloc Φ :
     (|==> ∃ γ, saved_pred3_own γ Φ)%I.
   Proof. apply saved_anything_alloc. Qed.
 
+  Lemma saved_pred3_agree γ Φ Ψ:
+    saved_pred3_own γ Φ -∗ saved_pred3_own γ Ψ -∗
+    ▷ (Φ ≡ Ψ).
+  Proof.
+    iIntros "HΦ HΨ /=".
+    iDestruct (saved_anything_agree with "HΦ HΨ") as "Heq".
+    destruct Φ, Ψ; rewrite /pack.
+    iApply bi.later_equivI; iApply "Heq".
+  Qed.
+
+  Lemma same_arity {Φ Ψ : packedFun} {n} :
+    Φ ≡{n}≡ Ψ → packedFun_arity Φ = packedFun_arity Ψ.
+  Proof. destruct Φ, Ψ. by case. Qed.
+
+  Lemma eq_ext (Φ Ψ : packedFun) : Φ ≡ Ψ ⊢ ⌜ ∃ n, Φ ≡{n}≡ Ψ ⌝: iProp Σ.
+  Proof. unseal; constructor => n x Hx /=. by exists n. Qed.
+
+  Lemma pred_impl (Φ Ψ : packedFun) n (Heq: Φ ≡{n}≡ Ψ)
+    (a : vec (packedFun_arity Φ) vl) b c:
+    unpack Φ a b c ≡{n}≡ unpack Ψ (rew [λ n, vec n vl] (same_arity Heq) in a) b c.
+  Proof.
+    move: (same_arity Heq) => HeqN. destruct Φ, Ψ; simpl in *.
+    case: Heq => /= Heq1.
+    have {HeqN} ->: HeqN = Heq1. exact: proof_irrel.
+    destruct Heq1; cbn => H. exact: H.
+  Qed.
+
+  Lemma eq_1 (Φ Ψ : packedFun) : Φ ≡ Ψ -∗ ⌜ packedFun_arity Φ = packedFun_arity Ψ ⌝: iProp Σ.
+  Proof.
+    iIntros "H".
+    iApply (internal_eq_rewrite _ _ (λ x, ⌜ packedFun_arity Φ = packedFun_arity x ⌝)%I with "H") => //.
+    move => n [/= ix ?] [/= iy ?] [/=]. intros ->. done.
+  Qed.
+
+  Lemma saved_pred3_agree_arity γ Φ Ψ:
+    saved_pred3_own γ Φ -∗ saved_pred3_own γ Ψ -∗
+    ▷ ⌜ packedFun_arity Φ = packedFun_arity Ψ ⌝.
+  Proof.
+    iIntros "HΦ HΨ /=".
+    iDestruct (saved_pred3_agree with "HΦ HΨ") as "Heq".
+    iNext. iApply (eq_1 with "Heq").
+  Qed.
+(*
   Lemma saved_pred3_agree γ Φ Ψ a b c:
     saved_pred3_own γ Φ -∗ saved_pred3_own γ Ψ -∗
+    ⌜ proj1_sig Φ ⌝
     ▷ (Φ a b c ≡ Ψ a b c).
   Proof.
     iIntros "HΦ HΨ /=".
@@ -90,10 +152,9 @@ Section saved_pred3.
     repeat setoid_rewrite bi.discrete_fun_equivI.
     iApply bi.later_equivI; iApply "Heq".
   Qed. *)
+
 End saved_pred3.
 
-(*
 Opaque saved_pred3_own.
 
 Notation "γ ⤇ φ" := (saved_pred3_own γ φ) (at level 20).
-*)
